examples/map/MapI0Mproof.v
@@ -34,9 +34,12 @@ Section SIMMODSEM.
   Let W: Type := Any.t * Any.t.
 
   Let wf: _ -> W -> Prop :=
-        @mk_wf _ unit
-               (fun _ st_src st_tgt =>
-                  ((∃ blk ofs l, ⌜st_src = l↑ /\ st_tgt = (Vptr blk ofs)↑⌝ ** OwnM ((blk, ofs) |-> (List.map Vint l)) ** pending0) ∨ (⌜st_src = ([]: list Z)↑⌝))%I).
+        @inv_wf
+          _ _
+          unit
+          (fun _ st_src st_tgt =>
+             ((∃ blk ofs l, ⌜st_src = l↑ /\ st_tgt = (Vptr blk ofs)↑⌝ ** OwnM ((blk, ofs) |-> (List.map Vint l)) ** pending0) ∨ (⌜st_src = ([]: list Z)↑⌝))%I)
+  .
 
   Variable GlobalStb: Sk.t -> gname -> option fspec.
   Hypothesis STBINCL: forall sk, stb_incl (to_stb MemStb) (GlobalStb sk).
@@ -67,7 +70,8 @@ Section SIMMODSEM.
     pending0 -∗ pending0 -∗ False%I.
   Proof.
     iIntros "H0 H1". iCombine "H0 H1" as "H".
-    iOwnWf "H". exfalso. rr in H1. clear - H1. admit "ez".
+    iOwnWf "H". exfalso. clear - H1.
+    rr in H1. ur in H1. unseal "ra". ss.
   Qed.
 
   Lemma points_to_get_split blk ofs l k v
@@ -122,331 +126,92 @@ Section SIMMODSEM.
     }
   Qed.
 
+  Lemma set_nth_map A B (f: A -> B) k l v
+    :
+    set_nth k (List.map f l) (f v) = option_map (List.map f) (set_nth k l v).
+  Proof.
+    revert k v. induction l; ss; i.
+    { destruct k; ss. }
+    { destruct k; ss. rewrite IHl. unfold option_map. des_ifs. }
+  Qed.
+
+  Lemma nth_error_map A B (f: A -> B) k l
+    :
+    nth_error (List.map f l) k = option_map f (nth_error l k).
+  Proof.
+    revert k. induction l; ss; i.
+    { destruct k; ss. }
+    { destruct k; ss. }
+  Qed.
+
   Theorem correct: refines2 [MapI0.Map] [MapM.Map GlobalStb].
   Proof.
     eapply adequacy_local2. econs; ss. i. rr.
-    econstructor 1 with (wf:=wf) (le:=top2); ss; et; swap 2 3.
-    { esplits. rr. econs; ss. eapply to_semantic. iIntros "_". iRight. auto. }
+    econstructor 1 with (wf:=wf) (le:=inv_le top2); ss; et; cycle 2.
+    { eexists (inl tt). rr. econs; ss. eapply to_semantic. iIntros "_". iRight. auto. }
+    { eapply inv_le_PreOrder. ss. }
     econs; ss.
-    { unfold MapI0.initF, MapM.initF, ccallU. init. harg. mDesAll. subst.
+    { unfold MapI0.initF, MapM.initF, ccallU. init. iarg. mDesAll. subst.
       mDesOr "INV".
       { mDesAll. subst. mAssertPure False; ss. iApply (pending0_unique with "A1 A"). }
       mDesAll. subst. steps. astart 100. acatch.
       { eapply STBINCL. stb_tac. ss. }
-      hcall _ _ with "".
-      { iModIntro. iSplitL.
-        { iRight. ss. }
-        instantiate (1:=Some _). ss. iPureIntro.
+      icall_open _ with "".
+      { iModIntro. instantiate (1:=Some _). ss. iPureIntro.
         splits; ss. admit "add range condition".
       }
       { ss. }
-      ss. mDesAll. subst.
-      { mDesOr "INV".
-        { mDesAll. subst. mAssertPure False; ss. iApply (pending0_unique with "A2 A"). }
-        mDesAll. subst. steps. astop. steps.
-        hret _; ss.
-        iModIntro. iSplit.
-        { iLeft. iSplits. iSplitR "A"; eauto. iSplit; eauto.
-          admit "malloc -> calloc".
-        }
-        { iSplits; eauto. }
+      ss. mDesAll. subst. steps. astop. steps.
+      iret _; ss.
+      iModIntro. iSplit.
+      { iLeft. iSplits. iSplitR "A"; eauto. iSplit; eauto.
+        admit "malloc -> calloc".
       }
+      { iSplits; eauto. }
     }
     econs; ss.
-    { unfold MapI0.setF, MapM.setF, ccallU. init. harg. mDesAll. subst.
+    { unfold MapI0.setF, MapM.setF, ccallU. init. iarg. mDesAll. subst.
       mDesOr "INV".
-      2:{ mDesAll. subst. steps. astop. steps. des_ifs. }
+      2:{ mDesAll. subst. steps. exfalso. des_ifs. }
       mDesAll. des. steps. unfold scale_int. des_ifs.
       2:{ admit "add int allignment condition". }
       steps. astart 1. acatch.
       { eapply STBINCL. stb_tac. ss. }
-      hcall _ _ with "".
-      { iModIntro. iSplitR.
-        { iLeft. ss. }
-        instantiate (1:=Some _). ss. iPureIntro.
-        splits; ss. admit "add range condition".
+      mApply points_to_set_split "A1".
+      2:{ rewrite set_nth_map. rewrite _UNWRAPU0. ss. }
+      mDesAll.
+      icall_open _ with "A1".
+      { iModIntro. instantiate (1:=Some (_, _, _)). ss.
+        iExists _. iSplit; eauto.
+        instantiate (1:=a2). admit "alignment".
       }
       { ss. }
-      ss. mDesAll. subst.
-      { mDesOr "INV".
-        { mDesAll. subst. mAssertPure False; ss. iApply (pending0_unique with "A2 A"). }
-        mDesAll. subst. steps. astop. steps.
-        hret _; ss.
-        iModIntro. iSplit.
-        { iLeft. iSplits. iSplitR "A"; eauto. iSplit; eauto.
-          admit "malloc -> calloc".
-        }
-        { iSplits; eauto. }
-      }
-
-steps. .ired_l. _step.
-      { ired_both. _step. des_ifs_safe. steps. force_l. steps.
-
- force_l. force_r.
-      {
-
-subst. steps. astop. steps. ired_l. steps. force_l. force_r.
-      {
-
-      subst. force_r. _step. steps. astart 10. steps.
-
-red in WF. inv WF.
-
-astop. steps. des_ifs. }
-
-
+      ss. mDesAll. subst. steps. astop. steps.
+      iret _; ss. iModIntro. iSplit; ss.
+      iLeft. iExists _. iExists _, _. iSplitR "A"; eauto.
+      iSplit; eauto. iApply "A2". admit "alignment".
     }
-
-mDesAll. subst. mAssertPure False; ss. iApply (pending0_unique with "A1 A"). }
-      mDesAll. subst. steps. astart 100. acatch.
+    econs; ss.
+    { unfold MapI0.getF, MapM.getF, ccallU. init. iarg. mDesAll. subst.
+      mDesOr "INV".
+      2:{ mDesAll. subst. steps. exfalso. destruct (Z.to_nat z); ss. }
+      mDesAll. des. steps. unfold scale_int. des_ifs.
+      2:{ admit "add int allignment condition". }
+      steps. astart 1. acatch.
       { eapply STBINCL. stb_tac. ss. }
-      hcall _ _ with "".
-      { iModIntro. iSplitL.
-        { iRight. ss. }
-        instantiate (1:=Some _). ss. iPureIntro.
-        splits; ss. admit "add range condition".
+      mApply points_to_get_split "A1".
+      2:{ eapply map_nth_error. eauto. }
+      mDesAll.
+      icall_open _ with "A1".
+      { iModIntro. instantiate (1:=Some (_, _, _)). ss.
+        iSplit; eauto. instantiate (1:=Vint z0). admit "alignment".
       }
       { ss. }
-      ss. mDesAll. subst.
-      { mDesOr "INV".
-        { mDesAll. subst. mAssertPure False; ss. iApply (pending0_unique with "A2 A"). }
-        mDesAll. subst. steps. astop. steps.
-        hret _; ss.
-        iModIntro. iSplit.
-        { iLeft. iSplits. iSplitR "A"; eauto. iSplit; eauto.
-          admit "malloc -> calloc".
-        }
-        { iSplits; eauto. }
-      }
+      ss. mDesAll. subst. steps. astop. steps.
+      iret _; ss. iModIntro. iSplit; ss.
+      iLeft. iExists _. iExists _, _. iSplitR "A"; eauto.
+      iSplit; eauto. iApply "A2". admit "alignment".
     }
-    {
-
-
-iSplits; eauto.
-iLeft.
-
-        { mDe
-
-
-eauto. eauto.
-
-        {
-
-
-      }
-
-
-stbtac.
-
-steps.
-      hcall _ _ with "".
-
-      unfold
-ss.
-
-
-
- sim_modsem: ModSemPair.sim MapM.MapSem (Stack1.StackSem global_stb) Stack0.StackSem.
-  Proof.
-    econstructor 1 with (wf:=wf) (le:=top2); ss; et; swap 2 3.
-    { esplits. econs; ss. eapply to_semantic. iIntros "H". iClear "H". iSplits; ss. }
-    econs; ss.
-    { unfold newF. init. harg. fold wf. mDesAll; des; subst. ss.
-      unfold new_body. steps. unfold ccallN, ccallU, cfunN, cfunU. steps.
-
-      astart 2. acatch. { eapply STBINCL. stb_tac; ss. } hcall (Some _) _ with "SIM"; ss; et.
-      { iModIntro. iSplits; ss; et.
-        { instantiate (1:=1%nat). ss. }
-        { iPureIntro. unfold_modrange_64. ss. }
-      }
-      Ltac post_call :=
-        fold wf; clear_fast; mDesAll; des_safe; subst; try rewrite Any.upcast_downcast in *; clarify; renamer.
-      post_call. rename a0 into handle.
-      steps.
-      force_r.
-      { ss. }
-      steps.
-
-      acatch. { eapply STBINCL. stb_tac; ss. } hcall (Some (_, _, _)) _ with "SIM A"; ss; et.
-      { iModIntro. iSplitL "SIM"; ss.
-        { iSplits; ss; et. }
-        { iSplits; ss; et. }
-      }
-      post_call. steps.
-      astop. steps.
-
-      force_l. exists handle. steps.
-      destruct (stk_mgr0 !! handle) eqn:T.
-      { mAssertPure False; ss.
-        (*** IEXPLOIT*) iDestruct (big_sepM_lookup_acc with "SIM") as "[B C]"; et. iDestruct "B" as (x) "[B D]".
-        iApply (points_to_disj with "POST B"); et.
-      }
-      astop. steps. astop. steps. force_l; ss. steps. astop. steps.
-
-      hret _; ss.
-      { iModIntro. iSplits; ss; et. iApply big_sepM_insert; ss. iFrame; ss; et. }
-      (*** ISPECIALIZE SYNTAX: iSpecialize ("A" $! _ _ H0). et. *)
-    }
-    econs; ss.
-    { unfold popF. init. harg. fold wf. mDesAll; des; subst. ss.
-      unfold pop_body, ccallU, cfunU.
-      steps. astop. steps. astop. steps. astop. steps. astart 7.
-
-      hide_k. destruct v; ss. des_ifs. clear_fast.
-      renamer. rename n into handle. rename l into stk. rename _UNWRAPU into T.
-      mAssert _ with "SIM".
-      { iDestruct (big_sepM_delete with "SIM") as "[B C]"; et. (* big_sepM_lookup_acc *)
-        instantiate (1:=_ ** _). iSplitL "B". { iExact "B". } iExact "C". }
-      mDesAll; ss. rename a into hd. renamer.
-
-      acatch. { eapply STBINCL. stb_tac; ss. } hcall (Some (_, _, _)) _ with "SIM A"; ss; et.
-      { iModIntro. iSplitL "SIM"; ss; et. }
-      post_call. unhide_k. steps.
-      hide_k.
-
-      force_r.
-      { mAssertPure _.
-        { iClear "SIM". iClear "POST". iApply is_list_wf. iApply "A2". }
-        des; clarify; et. des_ifs.
-      }
-      steps.
-
-      destruct stk as [|x stk1]; ss.
-      - mDesAll. subst.
-        unhide_k. steps. hide_k.
-        acatch. { eapply STBINCL. stb_tac; ss. } hcall (Some (_, _)) _ with "SIM POST"; ss.
-        { iModIntro. iSplitL "SIM"; ss; [et|]. iSplits; ss. repeat iRight. et. }
-        post_call. unhide_k. steps. astop. steps.
-        force_r.
-        { ss. }
-        steps. astop. steps. astop. steps.
-
-        hret _; ss. iModIntro. iSplits; ss; et.
-        destruct (stk_mgr1 !! handle) eqn:U.
-        { iExFalso. iDestruct (big_sepM_lookup_acc with "SIM") as "[B C]"; et. iDestruct "B" as (x) "[SIM B]".
-          iApply (points_to_disj with "POST1 SIM"). }
-        iApply big_sepM_insert; ss. iSplitR "SIM"; et.
-      - mDesAll. subst. rename a into hd. rename a0 into tl. rewrite points_to_split in ACC. mDesOwn "A1".
-        rewrite Z.add_0_l in *.
-        unhide_k. steps. hide_k.
-
-        acatch. { eapply STBINCL. stb_tac; ss. } hcall (Some (_, _)) _ with "SIM A1"; ss.
-        { iModIntro. iSplitL "SIM"; ss. { et. } iSplits; ss; et. }
-        post_call. unhide_k. steps.
-
-        force_r.
-        { ss. }
-        steps.
-
-        force_r.
-        { ss. }
-        steps.
-
-        unfold scale_int. uo. steps.
-        acatch. { eapply STBINCL. stb_tac; ss. } hcall (Some (_, _, _)) _ with "SIM POST1"; ss.
-        { iModIntro. iSplitL "SIM"; ss; et. }
-        post_call. steps.
-
-        acatch. { eapply STBINCL. stb_tac; ss. } hcall (Some (_, _, _)) _ with "SIM A2"; ss.
-        { iModIntro. iSplitL "SIM"; ss; et. }
-        post_call. steps.
-
-        acatch. { eapply STBINCL. stb_tac; ss. } hcall (Some (_, _)) _ with "SIM POST2"; ss.
-        { iModIntro. iSplitL "SIM"; ss; et. }
-        post_call. steps.
-
-        acatch. { eapply STBINCL. stb_tac; ss. } hcall (Some (_, _)) _ with "SIM POST1"; ss.
-        { iModIntro. iSplitL "SIM"; ss; et. }
-        post_call. steps.
-
-        acatch. { eapply STBINCL. stb_tac; ss. } hcall (Some (_, _, _)) _ with "SIM POST"; ss.
-        { iModIntro. iSplitL "SIM"; ss; et. }
-        post_call. steps.
-
-        astop. steps. unfold pget. steps. renamer.
-
-        destruct (stk_mgr1 !! handle) eqn:V.
-        { mAssertPure False; ss. iDestruct (big_sepM_lookup_acc with "SIM") as "[B C]"; et.
-          iDestruct "B" as (y) "[SIM B]".
-          iApply (points_to_disj with "POST1 SIM"). }
-        steps. astop. steps. astop. steps.
-
-        hret _; ss.
-        { iModIntro. iSplits; ss; et. iApply big_sepM_insert; ss. iFrame. iExists _; ss. iFrame. }
-    }
-    econs; ss.
-    { unfold pushF. init. harg. fold wf. mDesAll; des; subst. ss.
-      unfold push_body, ccallU, cfunU.
-      steps. astop. steps. astop. steps. astop. steps. astart 7.
-
-      hide_k. destruct v; ss. des_ifs. clear_tac.
-      rename n into handle. renamer. rename l into stk. rename _UNWRAPU into T.
-      mAssert _ with "SIM".
-      { iDestruct (big_sepM_delete with "SIM") as "[B C]"; et. (* big_sepM_lookup_acc *)
-        instantiate (1:=_ ** _). iSplitL "B". { iExact "B". } iExact "C". }
-      mDesAll; ss. renamer. rename a into hd.
-
-      acatch. { eapply STBINCL. stb_tac; ss. } hcall (Some _) _ with "SIM"; ss; et.
-      { iModIntro. iSplitL "SIM"; et. iSplits; ss; et.
-        { instantiate (1:=2). ss. }
-        { iPureIntro. ss. }
-      }
-      post_call. rename a0 into node. unhide_k. steps.
-
-      rewrite points_to_split in ACC. mDesOwn "A1". rewrite Z.add_0_l in *. clear_fast.
-
-      unfold scale_int. uo. steps.
-
-      force_r; ss. steps.
-
-      acatch. { eapply STBINCL. stb_tac; ss. } hcall (Some (_, _, _)) _ with "A SIM"; ss; et.
-      { iModIntro. iSplitL "SIM"; et. }
-      post_call. steps.
-
-      acatch. { eapply STBINCL. stb_tac; ss. } hcall (Some (_, _, _)) _ with "A1 SIM"; ss; et.
-      { iModIntro. iSplitL "SIM"; et. }
-      post_call. steps.
-
-      acatch. { eapply STBINCL. stb_tac; ss. } hcall (Some (_, _, _)) _ with "A3 SIM"; ss; et.
-      { iModIntro. iSplitL "SIM"; et. }
-      post_call. steps.
-
-      acatch. { eapply STBINCL. stb_tac; ss. } hcall (Some (_, _, _)) _ with "POST SIM"; ss; et.
-      { iModIntro. iSplitL "SIM"; et. }
-      post_call. steps.
-
-      astop. steps.
-
-      destruct (stk_mgr1 !! handle) eqn:V.
-      { mAssertPure False; ss. iDestruct (big_sepM_lookup_acc with "SIM") as "[B C]"; et.
-        iDestruct "B" as (y) "[SIM B]". iApply (points_to_disj with "POST3 SIM"). }
-
-      hret _; ss.
-      { iModIntro. iSplits; ss; et.
-        iApply big_sepM_insert; ss. iFrame. iExists _; ss. iFrame.
-        iExists _, _. iFrame. iSplit; ss. erewrite points_to_split with (hd:=v0) (tl:=[hd]).
-        iSplitL "POST1"; et.
-      }
-    }
-  Unshelve.
-    all: try exact 0. all: ss.
+    Unshelve. all: ss.
   Qed.
-
 End SIMMODSEM.
-
-
-
-Section SIMMOD.
-
-  Context `{Σ: GRA.t}.
-  Context `{@GRA.inG memRA Σ}.
-
-  Variable global_stb: Sk.t -> gname -> option fspec.
-  Hypothesis STBINCL: forall sk, stb_incl (to_stb (StackStb ++ MemStb)) (global_stb sk).
-
-  Theorem correct: refines2 [Stack0.Stack] [Stack1.Stack global_stb].
-  Proof.
-    eapply adequacy_local2. econs; ss. ii. eapply sim_modsem; ss.
-  Qed.
-
-End SIMMOD.
